Foundation/IntProp/Kripke/LEM.lean
@@ -12,58 +12,80 @@ namespace LO.IntProp
 open System
 open Formula Formula.Kripke
 
-namespace Kripke
-
-abbrev twopointsFrame : Kripke.Frame where
-  World := Unit ⊕ Unit
-  Rel x y :=
-    match x, y with
-    | .inl _, .inl _ => True
-    | .inr _, .inr _ => True
-    | .inl _, .inr _ => True
-    | _, _ => False
-  trans_Rel := by simp [Transitive];
-  refl_Rel := by simp [Reflexive];
-
-namespace twopoints
-
-lemma is_transitive : Transitive twopointsFrame := twopointsFrame.trans_Rel
-lemma is_reflexive : Reflexive twopointsFrame := twopointsFrame.refl_Rel
-lemma is_confluent : Confluent twopointsFrame := by simp [Confluent]
-lemma is_connected : Connected twopointsFrame := by simp [Connected]
-
-lemma noLEM {a : α} : ¬(twopointsFrame#α ⊧ (atom a) ⋎ ∼(atom a)) := by
-  simp only [Semantics.Realize, ValidOnFrame];
-  push_neg;
-  use (λ w _ => match w with | .inr _ => True | .inl _ => False), by simp;
-  simp [Semantics.Realize, ValidOnModel, Satisfies];
-
-end twopoints
-
-end Kripke
-
-
-variable {a : α}
-
 namespace Hilbert
 
-theorem Int.noLEM : (Hilbert.Int α) ⊬ (atom a) ⋎ ∼(atom a) := by
+theorem Int.no_WeakLEM : (Hilbert.Int ℕ) ⊬ Axioms.WeakLEM (atom a) := by
   by_contra hC;
-  apply Kripke.twopoints.noLEM;
-  apply Kripke.sound.sound hC;
-  tauto;
+  let F : Kripke.Frame := {
+    World := Fin 3,
+    Rel := λ x y =>
+      match x, y with
+      | 0, x => True
+      | x, y => x = y,
+    rel_po := {
+      refl := by aesop;
+      antisymm := by aesop;
+      trans := by aesop;
+    }
+  };
+  have : F ⊧ Axioms.WeakLEM (atom a) := Kripke.sound.sound hC F $ by tauto;
+  have : Confluent F := by sorry;
+  have : ¬Confluent F := by
+    simp only [Confluent]; push_neg;
+    use 0, 1, 2;
+    simp;
+  contradiction;
 
-theorem Int_strictly_weaker_than_Cl [Inhabited α] : (Hilbert.Int α) <ₛ (Hilbert.Cl α) := by
+theorem Int_strictly_weaker_than_LC : (Hilbert.Int ℕ) <ₛ (Hilbert.KC ℕ) := by
   constructor;
-  . exact Hilbert.Int_weaker_than_Cl;
+  . exact Hilbert.Int_weaker_than_KC;
   . apply weakerThan_iff.not.mpr;
     push_neg;
-    use (atom default) ⋎ ∼(atom default);
+    use ∼(atom default) ⋎ ∼∼(atom default);
     constructor;
-    . exact lem!;
-    . exact Int.noLEM;
+    . exact wlem!;
+    . exact Int.no_WeakLEM;
 
+/-
+theorem KC.no_Dummet : (Hilbert.KC ℕ) ⊬ Axioms.GD (atom a) (atom b) := by
+  by_contra hC;
+  let F : Kripke.Frame := {
+    World := Fin 4,
+    Rel := λ x y =>
+      match x, y with
+      | 1, 2 => False
+      | x, y => x ≤ y
+    rel_po := {
+      refl := by aesop;
+      antisymm := by sorry;
+      trans := by
+        intro x y z;
+        aesop;
+        match y with
+        | 0 => simp; rintro rfl; tauto;
+        | 1 =>
+          match x with
+          | 0 => sorry;
+          | 1 => aesop;
+          | _ => sorry;
+        | 2 => sorry;
+        | 3 => simp; rintro _ rfl; tauto;
+        -- match (x, y, z) with
+        -- | 0, 1, 2 => simp;
+        -- | _ => sorry;
+    }
+  };
+  have : F ⊧ Axioms.GD (atom a) (atom b) := Kripke.sound.sound hC F $ by
+    simp [Confluent];
+    intro x y z Rxy Ryz;
+    match x, y, z with
+    | 0, 1, 2 => use 3;
+    | 0, 2, 1 => use 3;
+    | 1, 3, 2 => use 0;
+    | _, _, _ => sorry;
+-/
 
+/-
 theorem KC.noLEM : (Hilbert.KC α) ⊬ (atom a) ⋎ ∼(atom a) := by
   by_contra hC;
   apply Kripke.twopoints.noLEM;
@@ -79,23 +101,47 @@ theorem KC_strictly_weaker_than_Cl [Inhabited α] : (Hilbert.KC α) <ₛ (Hilber
     constructor;
     . exact lem!;
     . exact KC.noLEM;
+-/
+lemma KC.no_dummett : (Hilbert.KC ℕ) ⊬ Axioms.Dummett (atom a) (atom b) := by sorry;
 
+theorem KC_strictly_weaker_than_LC : (Hilbert.KC ℕ) <ₛ (Hilbert.LC ℕ) := by
+  constructor;
+  . sorry;
+  . apply weakerThan_iff.not.mpr;
+    push_neg;
+    use Axioms.Dummett (atom 0) (atom 1);
+    constructor;
+    . exact dummett!;
+    . exact KC.no_dummett;
 
-theorem LC.noLEM : (Hilbert.LC α) ⊬ (atom a) ⋎ ∼(atom a) := by
+theorem LC.no_LEM : (Hilbert.LC ℕ) ⊬ Axioms.LEM (atom a) := by
   by_contra hC;
-  apply Kripke.twopoints.noLEM;
-  apply Kripke.sound.sound hC;
-  exact Kripke.twopoints.is_connected;
+  let F : Kripke.Frame := {
+    World := Fin 2,
+    Rel := λ x y => x ≤ y
+  };
+  have : F ⊧ Axioms.LEM (atom a) := Kripke.sound.sound hC F $ by
+    simp [Connected];
+    omega;
+  have : Euclidean F := by sorry;
+  have : ¬Euclidean F := by
+    simp only [Euclidean]; push_neg;
+    use 0, 0, 1;
+    simp;
+  contradiction;
 
-theorem LC_strictly_weaker_than_Cl [DecidableEq α] [Inhabited α] : (Hilbert.LC α) <ₛ (Hilbert.Cl α) := by
+theorem LC_strictly_weaker_than_Cl : (Hilbert.LC ℕ) <ₛ (Hilbert.Cl ℕ) := by
   constructor;
   . exact Hilbert.LC_weaker_than_Cl;
   . apply weakerThan_iff.not.mpr;
     push_neg;
-    use (atom default) ⋎ ∼(atom default);
+    use Axioms.LEM (atom 0);
     constructor;
     . exact lem!;
-    . exact LC.noLEM;
+    . exact LC.no_LEM;
+
+theorem Int_strictly_weaker_than_Cl : (Hilbert.Int ℕ) <ₛ (Hilbert.Cl ℕ) :=
+  strictlyWeakerThan.trans Int_strictly_weaker_than_LC $ strictlyWeakerThan.trans KC_strictly_weaker_than_LC LC_strictly_weaker_than_Cl
 
 end Hilbert
 
